finer grained preprocessing of step theorems
Make "computation" of memory containing instruction machine specific.
This simplifies the code, there is now now fancy computation needed.
This allows changing the theorem more, by e.g. applying arithmetic
simplifications which would interfer with the fancy computation.

As a result, the code is more rebust, but incidentially also much faster
and simpler. This is a necessary preparation for instantiating the PC
late and for lifting stores.

src/tools/lifter/bir_inst_liftingLib.sml
@@ -33,8 +33,6 @@ val block_observe_ty = mk_vartype ":'observation_type"
 val bir_is_lifted_inst_block_COMPUTE_block_tm =
    inst [Type.alpha |-> block_observe_ty] (get_const "bir_is_lifted_inst_block_COMPUTE_block")
 
-val bmr_ms_mem_contains_tm = get_const "bmr_ms_mem_contains";
-
 val bir_is_lifted_inst_block_COMPUTE_precond_tm =
     inst [Type.delta |-> block_observe_ty] (get_const "bir_is_lifted_inst_block_COMPUTE_precond")
 
@@ -207,11 +205,14 @@ functor bir_inst_liftingFunctor (MD : sig val mr : bmr_rec end) : bir_inst_lifti
 
 
   (* Construct the extra thms *)
-  val ms_extra_REWRS = let
+  val ms_extra_REWRS0 = let
      val thm0 = SPECL [bs_v, ms_v] (ISPEC (#bmr_const mr) bmr_rel_implies_extra)
      val thm1 = UNDISCH thm0
-     val thm2 = SIMP_RULE (std_ss) [bmr_eval_REWRS] thm1
-  in thm2 end;
+  in thm1 end;
+
+  val ms_extra_REWRS =
+     SIMP_RULE (std_ss) [bmr_eval_REWRS] ms_extra_REWRS0;
+
 
 
   (* preinstantiated bmr_ms_mem_contains term *)
@@ -302,61 +303,23 @@ functor bir_inst_liftingFunctor (MD : sig val mr : bmr_rec end) : bir_inst_lifti
        raise (bir_inst_liftingExn (hex_code, BILED_msg "label thm failed"));
 
      (* Normalise all resulting theorems *)
-     fun norm_thm thm =
-        SIMP_RULE std_ss [pc_thm, ms_extra_REWRS, satTheory.AND_IMP,
-           alignmentTheory.aligned_numeric, wordsTheory.word_add_n2w] thm handle UNCHANGED => thm
+     fun norm_thm thm = let
+        val thm0 = HYP_CONV_RULE (K true) (PURE_REWRITE_CONV [pc_thm]) thm
+        val thm1 = PROVE_HYP ms_extra_REWRS0 thm0
+        val thm2 = SIMP_RULE std_ss [pc_thm, ms_extra_REWRS, satTheory.AND_IMP,
+           alignmentTheory.aligned_numeric, wordsTheory.word_add_n2w] thm1 handle UNCHANGED => thm1
+     in
+        thm2
+     end
      val lifted_thms = map norm_thm lifted_thms_raw;
 
-     (* try to compute bmr_ms_mem_contains *)
-     val (mm_tm, mm_thm) = let
-       (* first get the common preconds *)
-       val common_preconds = let
-          fun preconds_of_thm thm =
-            HOLset.addList (empty_tmset, fst (strip_imp_only (concl thm)))
-
-          val preconds = foldl (fn (thm, s) => HOLset.intersection (s, preconds_of_thm thm))
-             (preconds_of_thm (hd lifted_thms)) (tl lifted_thms)
-          in HOLset.listItems preconds end
-
-       (* the extract pairs of mem address and values *)
-       val mem_precond_pairs = Lib.mapfilter (fn tm => let
-          val (l_tm, v_tm) = dest_eq tm;
-          val (ms_t, a_tm) = (#bmr_dest_mem mr) l_tm
-          val _ = assert (aconv ms_v) ms_t
-          val a_n = numSyntax.dest_numeral (fst (wordsSyntax.dest_n2w a_tm))
-       in (a_n, v_tm, tm) end) common_preconds
-       val _ = assert (not o List.null) mem_precond_pairs
-
-       (* sort it and try to combine *)
-       val sorted_mem_pairs = sort (fn (n1, _) => (fn (n2, _) => (Arbnum.< (n2, n1))))
-          (map (fn (a, v, _) => (a,v)) mem_precond_pairs)
-       val (n, vs) = foldl (fn ((n', v), (n, vs)) =>
-         if (Arbnum.plus1 n' = n) then (n', v::vs) else fail())
-         ((fn (n, v) => (n, [v])) (hd sorted_mem_pairs)) (tl sorted_mem_pairs)
-
-       (* make the term *)
-       val mm_tm = let
-          val addr_tm =  mk_mem_addr_from_num n;
-          val v_tm = listSyntax.mk_list (vs, type_of (hd vs))
-       in pairSyntax.mk_pair (addr_tm, v_tm) end;
-
-       (* show that this really implies all the preconds *)
-       val precond_thm = let
-         val p_tm = mk_comb (bmr_ms_mem_contains_tm_mr, mm_tm)
-         val c_tm = list_mk_conj (map (fn (_, _, tm) => tm) mem_precond_pairs)
-         val thm0 = prove (mk_imp (p_tm, c_tm),
-             SIMP_TAC (std_ss++bmr_ss++wordsLib.WORD_ARITH_ss) [
-                bmr_ms_mem_contains_def, bmr_mem_lf_def,
-                (#bmr_eval_thm mr)]);
-       in UNDISCH thm0 end;
-     in (mm_tm, precond_thm) end handle HOL_ERR _ =>
-       raise (bir_inst_liftingExn (hex_code, BILED_msg "mem region computation failed"));
-
-
-     (* Rewrite with these new mm theorems *)
-     val lifted_thms2 = map (REWRITE_RULE [mm_thm]) lifted_thms
+     (* try to get bmr_ms_mem_contains *)
+     val mm_tm = let
+       val (_, _, mm_tm) = Lib.tryfind dest_bmr_ms_mem_contains (hyp (hd lifted_thms))
+     in mm_tm end handle HOL_ERR _ =>
+       raise (bir_inst_liftingExn (hex_code, BILED_msg "mem region search failed"));
   in
-     (lifted_thms2, mm_tm, label_tm)
+     (lifted_thms, mm_tm, label_tm)
   end handle HOL_ERR _ =>
     raise (bir_inst_liftingExn (hex_code, BILED_msg "mk_inst_lifting_theorems failed"));
 
